theories/binary_format_parser.v
@@ -7,7 +7,7 @@ From compcert Require Import Integers.
 From parseque Require Import Parseque.
 From Coq.Strings Require Import Byte.
 From Wasm Require Import leb128.
-Require Import Coq.Arith.Le.
+Require Import PeanoNat.
 Require Import BinNat.
 
 Notation "p $> b" := (cmap b p) (at level 59, right associativity).
