theories/check_toks.v
@@ -1,6 +1,7 @@
 From compcert Require Import Integers.
 From parseque Require Import Parseque Running.
-Require Import Coq.Arith.Le.
+Require Import PeanoNat. 
+
 
 Section Check.
 
